SStructTT/Dynamic/Context.lean
@@ -5,9 +5,10 @@ namespace Dynamic
 variable {Srt : Type} [inst : SStruct Srt]
 
 abbrev Ctx Srt := List (Option (Tm Srt × Srt))
-notation m " :⟨" s "⟩" Δ => some (m, s) :: Δ
-notation "□" => none
+notation m " :⟨" s "⟩ " Δ => some (m, s) :: Δ
+notation "_:" Δ => none :: Δ
 
+@[scoped aesop safe [constructors]]
 inductive Merge : Ctx Srt -> Ctx Srt -> Ctx Srt -> Prop where
   | nil : Merge [] [] []
   | contra {Δ1 Δ2 Δ} A s :
@@ -16,40 +17,98 @@ inductive Merge : Ctx Srt -> Ctx Srt -> Ctx Srt -> Prop where
     Merge (A :⟨s⟩ Δ1) (A :⟨s⟩ Δ2) (A :⟨s⟩ Δ)
   | left {Δ1 Δ2 Δ} A s :
     Merge Δ1 Δ2 Δ ->
-    Merge (A :⟨s⟩ Δ1) (□ :: Δ2)   (A :⟨s⟩ Δ)
+    Merge (A :⟨s⟩ Δ1) (_: Δ2) (A :⟨s⟩ Δ)
   | right {Δ1 Δ2 Δ} A s :
     Merge Δ1 Δ2 Δ ->
-    Merge (□ :: Δ1) (A :⟨s⟩ Δ2) (A :⟨s⟩ Δ)
-  | implicit {Δ1 Δ2 Δ} :
+    Merge (_: Δ1) (A :⟨s⟩ Δ2) (A :⟨s⟩ Δ)
+  | im {Δ1 Δ2 Δ} :
     Merge Δ1 Δ2 Δ ->
-    Merge (□ :: Δ1) (□ :: Δ2) (□ :: Δ)
+    Merge (_: Δ1) (_: Δ2) (_: Δ)
 
-notation Δ1 " ∪ " Δ2 " => " Δ => Merge Δ1 Δ2 Δ
+@[scoped aesop safe [constructors]]
+inductive Lower : Ctx Srt -> Srt -> Prop where
+  | nil s : Lower [] s
+  | ex {Δ A s s'} :
+    s' ≤ s ->
+    Lower Δ s ->
+    Lower (A :⟨s'⟩ Δ) s
+  | im {Δ s} :
+    Lower Δ s ->
+    Lower (_: Δ) s
 
-inductive Key : Ctx Srt -> Srt -> Prop where
-  | nil s : Key [] s
-  | explicit Δ A s s0 :
-    s0 ≤ s ->
-    Key Δ s ->
-    Key (A :⟨s0⟩ Δ) s
-  | implicit Δ s :
-    Key Δ s ->
-    Key (□ :: Δ) s
+@[scoped aesop safe [constructors]]
+inductive Weak : Ctx Srt -> Prop where
+  | zero : Weak []
+  | ex {Δ A s} :
+    s ∈ weaken_set ->
+    Weak Δ ->
+    Weak (A :⟨s⟩ Δ)
+  | im {Δ} :
+    Weak Δ ->
+    Weak (_: Δ)
 
-notation Δ " ▹ " s => Key Δ s
+@[scoped aesop safe [constructors]]
+inductive Has : Ctx Srt -> Var -> Srt -> Tm Srt -> Prop where
+  | zero {Δ A s} :
+    Weak Δ ->
+    Has (A :⟨s⟩ Δ) 0 s A.[shift 1]
+  | ex {Δ A B x s s'} :
+    s' ∈ weaken_set ->
+    Has Δ x s A ->
+    Has (B :⟨s'⟩ Δ) (x + 1) s A.[shift 1]
+  | im {Δ A x s} :
+    Has Δ x s A ->
+    Has (_: Δ) (x + 1) s A.[shift 1]
 
-/-
-Inductive dyn_has : dyn_ctx -> var -> sort -> term -> Prop :=
-| dyn_has_O Δ A s :
-  Δ ▷ U ->
-  dyn_has (A .{s} Δ) 0 s A.[ren (+1)]
-| dyn_has_S Δ A B x s :
-  dyn_has Δ x s A ->
-  dyn_has (B :U Δ) x.+1 s A.[ren (+1)]
-| dyn_has_N Δ A x s :
-  dyn_has Δ x s A ->
-  dyn_has (_: Δ) x.+1 s A.[ren (+1)].
--/
+lemma Lower.split_s0 {Δ : Ctx Srt} :
+    Lower Δ s0 -> ∃ Δ1 Δ2, Lower Δ1 s0 ∧ Lower Δ2 s0 ∧ Merge Δ1 Δ2 Δ := by
+  generalize e: inst.s0 = s
+  intro l; induction l
+  case nil =>
+    subst_vars
+    exists [], []; aesop
+  case ex A _ s' h _ ih =>
+    subst_vars
+    have := inst.le_antisymm _ _ h (inst.s0_min s')
+    subst_vars
+    have ⟨Δ1, Δ2, l1, l2, mrg⟩ := ih rfl
+    exists A :⟨s0⟩ Δ1, A :⟨s0⟩ Δ2
+    and_intros
+    . constructor <;> assumption
+    . constructor <;> assumption
+    . constructor
+      apply inst.s0_contra
+      assumption
+  case im ih =>
+    subst_vars
+    have ⟨Δ1, Δ2, l1, l2, mrg⟩ := ih rfl
+    exists _: Δ1, _: Δ2
+    and_intros
+    . constructor; assumption
+    . constructor; assumption
+    . constructor; assumption
 
--- inductive Has : Ctx Srt -> Var -> Srt -> Tm Srt -> Prop where
---   | zero Δ A s
+lemma Merge.lower {Δ1 Δ2 Δ : Ctx Srt} s :
+    Merge Δ1 Δ2 Δ -> Lower Δ1 s -> Lower Δ2 s -> Lower Δ s := by
+  intro mrg; induction mrg
+  case nil =>
+    intros; constructor
+  case contra ih =>
+    intro l1 l2; cases l1; cases l2
+    apply Lower.ex
+    . assumption
+    . apply ih <;> assumption
+  case left ih =>
+    intro l1 l2; cases l1; cases l2
+    apply Lower.ex
+    . assumption
+    . apply ih <;> assumption
+  case right ih =>
+    intro l1 l2; cases l1; cases l2
+    apply Lower.ex
+    . assumption
+    . apply ih <;> assumption
+  case im ih =>
+    intro l1 l2; cases l1; cases l2
+    apply Lower.im
+    apply ih <;> assumption
