SStructTT/Static/Progress.lean
@@ -7,39 +7,48 @@ variable {Srt : Type} [inst : SStruct Srt]
 inductive Value : Tm Srt -> Prop where
   | var x : Value (.var x)
   | srt s i : Value (.srt s i)
-  | pi A B r s : Value (.pi A B r s)
-  | lam A m r s : Value (.lam A m r s)
-  | sig A B r s : Value (.sig A B r s)
-  | pair_im m n s :
+  | pi0 A B s : Value (.pi0 A B s)
+  | pi1 A B s : Value (.pi1 A B s)
+  | lam0 A m s : Value (.lam0 A m s)
+  | lam1 A m s : Value (.lam1 A m s)
+  | sig0 A B s : Value (.sig0 A B s)
+  | sig1 A B s : Value (.sig1 A B s)
+  | tup0 m n s :
     Value m ->
-    Value (.pair m n .im s)
-  | pair_ex m n s :
+    Value (.tup0 m n s)
+  | tup1 m n s :
     Value m ->
     Value n ->
-    Value (.pair m n .ex s)
+    Value (.tup1 m n s)
   | bool : Value .bool
   | tt : Value .tt
   | ff : Value .ff
   | idn A m n : Value (.idn A m n)
   | rfl m : Value (.rfl m)
 
-lemma Typed.pi_canonical {A B C m : Tm Srt} {r s} :
-    [] ⊢ m : C -> C === .pi A B r s -> Value m ->
-    ∃ A n, m = .lam A n r s := by
+lemma Typed.pi0_canonical {A B C m : Tm Srt} {s} :
+    [] ⊢ m : C -> C === .pi0 A B s -> Value m ->
+    ∃ A n, m = .lam0 A n s := by
   generalize e: [] = Γ
-  intro ty; induction ty generalizing A B r s
+  intro ty; induction ty generalizing A B s
   all_goals try trivial
   case srt => intro eq; false_conv eq
   case var hs _ => subst_vars; cases hs
-  case pi => intro eq; false_conv eq
-  case lam _ A0 B0 m _ _ _ _ _ _ _ _ =>
+  case pi0 => intro eq; false_conv eq
+  case pi1 => intro eq; false_conv eq
+  case lam0 _ A0 B0 m _ _ _ _ _ _ _ =>
     intro eq _
-    have ⟨_, _, _⟩ := Conv.pi_inj eq
+    have ⟨_, _, _⟩ := Conv.pi0_inj eq
     subst_vars; exists A0, m
-  case app => intro _ vl; cases vl
-  case sig => intro eq; false_conv eq
-  case proj => intro _ vl; cases vl
-  case pair => intro eq; false_conv eq
+  case lam1 => intro eq; false_conv eq
+  case app0 => intro _ vl; cases vl
+  case app1 => intro _ vl; cases vl
+  case sig0 => intro eq; false_conv eq
+  case sig1 => intro eq; false_conv eq
+  case tup0 => intro eq; false_conv eq
+  case tup1 => intro eq; false_conv eq
+  case proj0 => intro _ vl; cases vl
+  case proj1 => intro _ vl; cases vl
   case bool => intro eq; false_conv eq
   case tt => intro eq; false_conv eq
   case ff => intro eq; false_conv eq
@@ -54,23 +63,103 @@ lemma Typed.pi_canonical {A B C m : Tm Srt} {r s} :
     . apply Conv.trans <;> assumption
     . assumption
 
-lemma Typed.sig_canonical {A B C m : Tm Srt} {r s} :
-    [] ⊢ m : C -> C === .sig A B r s -> Value m ->
-    ∃ m1 m2, m = .pair m1 m2 r s := by
+lemma Typed.pi1_canonical {A B C m : Tm Srt} {s} :
+    [] ⊢ m : C -> C === .pi1 A B s -> Value m ->
+    ∃ A n, m = .lam1 A n s := by
   generalize e: [] = Γ
-  intro ty; induction ty generalizing A B r s
+  intro ty; induction ty generalizing A B s
   all_goals try trivial
   case srt => intro eq; false_conv eq
   case var hs _ => subst_vars; cases hs
-  case pi => intro eq; false_conv eq
-  case lam => intro eq; false_conv eq
-  case app => intro _ vl; cases vl
-  case sig => intro eq; false_conv eq
-  case proj => intro _ vl; cases vl
-  case pair _ A0 B0 m n _ _ _ _ _ _ _ _ _ =>
+  case pi0 => intro eq; false_conv eq
+  case pi1 => intro eq; false_conv eq
+  case lam0 => intro eq; false_conv eq
+  case lam1 _ A0 B0 m _ _ _ _ _ _ _ =>
     intro eq _
-    have ⟨_, _, _⟩ := Conv.sig_inj eq
+    have ⟨_, _, _⟩ := Conv.pi1_inj eq
+    subst_vars; exists A0, m
+  case app0 => intro _ vl; cases vl
+  case app1 => intro _ vl; cases vl
+  case sig0 => intro eq; false_conv eq
+  case sig1 => intro eq; false_conv eq
+  case tup0 => intro eq; false_conv eq
+  case tup1 => intro eq; false_conv eq
+  case proj0 => intro _ vl; cases vl
+  case proj1 => intro _ vl; cases vl
+  case bool => intro eq; false_conv eq
+  case tt => intro eq; false_conv eq
+  case ff => intro eq; false_conv eq
+  case ite => intro _ vl; cases vl
+  case idn => intro eq; false_conv eq
+  case rfl => intro eq; false_conv eq
+  case rw => intro _ vl; cases vl
+  case conv ihm _ =>
+    intro eq vl
+    apply ihm
+    . assumption
+    . apply Conv.trans <;> assumption
+    . assumption
+
+lemma Typed.sig0_canonical {A B C m : Tm Srt} {s} :
+    [] ⊢ m : C -> C === .sig0 A B s -> Value m ->
+    ∃ m1 m2, m = .tup0 m1 m2 s := by
+  generalize e: [] = Γ
+  intro ty; induction ty generalizing A B s
+  all_goals try trivial
+  case srt => intro eq; false_conv eq
+  case var hs _ => subst_vars; cases hs
+  case pi0 => intro eq; false_conv eq
+  case pi1 => intro eq; false_conv eq
+  case lam0 => intro eq; false_conv eq
+  case lam1 => intro eq; false_conv eq
+  case app0 => intro _ vl; cases vl
+  case app1 => intro _ vl; cases vl
+  case sig0 => intro eq; false_conv eq
+  case sig1 => intro eq; false_conv eq
+  case tup0 _ A0 B0 m n _ _ _ _ _ _ _ _ =>
+    intro eq _
+    have ⟨_, _, _⟩ := Conv.sig0_inj eq
     subst_vars; exists m, n
+  case tup1 => intro eq; false_conv eq
+  case proj0 => intro _ vl; cases vl
+  case proj1 => intro _ vl; cases vl
+  case bool => intro eq; false_conv eq
+  case tt => intro eq; false_conv eq
+  case ff => intro eq; false_conv eq
+  case ite => intro _ vl; cases vl
+  case idn => intro eq; false_conv eq
+  case rfl => intro eq; false_conv eq
+  case rw => intro _ vl; cases vl
+  case conv ihm _ =>
+    intro eq vl
+    apply ihm
+    . assumption
+    . apply Conv.trans <;> assumption
+    . assumption
+
+lemma Typed.sig1_canonical {A B C m : Tm Srt} {s} :
+    [] ⊢ m : C -> C === .sig1 A B s -> Value m ->
+    ∃ m1 m2, m = .tup1 m1 m2 s := by
+  generalize e: [] = Γ
+  intro ty; induction ty generalizing A B s
+  all_goals try trivial
+  case srt => intro eq; false_conv eq
+  case var hs _ => subst_vars; cases hs
+  case pi0 => intro eq; false_conv eq
+  case pi1 => intro eq; false_conv eq
+  case lam0 => intro eq; false_conv eq
+  case lam1 => intro eq; false_conv eq
+  case app0 => intro _ vl; cases vl
+  case app1 => intro _ vl; cases vl
+  case sig0 => intro eq; false_conv eq
+  case sig1 => intro eq; false_conv eq
+  case tup0 => intro eq; false_conv eq
+  case tup1 _ A0 B0 m n _ _ _ _ _ _ _ _ =>
+    intro eq _
+    have ⟨_, _, _⟩ := Conv.sig1_inj eq
+    subst_vars; exists m, n
+  case proj0 => intro _ vl; cases vl
+  case proj1 => intro _ vl; cases vl
   case bool => intro eq; false_conv eq
   case tt => intro eq; false_conv eq
   case ff => intro eq; false_conv eq
@@ -92,12 +181,18 @@ lemma Typed.bool_canonical {C m : Tm Srt} :
   all_goals try trivial
   case srt => intro eq; false_conv eq
   case var hs _ => subst_vars; cases hs
-  case pi => intro eq; false_conv eq
-  case lam => intro eq; false_conv eq
-  case app => intro _ vl; cases vl
-  case sig => intro eq; false_conv eq
-  case proj => intro _ vl; cases vl
-  case pair => intro eq; false_conv eq
+  case pi0 => intro eq; false_conv eq
+  case pi1 => intro eq; false_conv eq
+  case lam0 => intro eq; false_conv eq
+  case lam1 => intro eq; false_conv eq
+  case app0 => intro _ vl; cases vl
+  case app1 => intro _ vl; cases vl
+  case sig0 => intro eq; false_conv eq
+  case sig1 => intro eq; false_conv eq
+  case tup0 => intro eq; false_conv eq
+  case tup1 => intro eq; false_conv eq
+  case proj0 => intro _ vl; cases vl
+  case proj1 => intro _ vl; cases vl
   case bool => intro eq; false_conv eq
   case tt => intros; left; rfl
   case ff => intros; right; rfl
@@ -119,12 +214,18 @@ lemma Typed.idn_canonical {A C m a b : Tm Srt} :
   all_goals try trivial
   case srt => intro eq; false_conv eq
   case var hs _ => subst_vars; cases hs
-  case pi => intro eq; false_conv eq
-  case lam => intro eq; false_conv eq
-  case app => intro _ vl; cases vl
-  case sig => intro eq; false_conv eq
-  case proj => intro _ vl; cases vl
-  case pair => intro eq; false_conv eq
+  case pi0 => intro eq; false_conv eq
+  case pi1 => intro eq; false_conv eq
+  case lam0 => intro eq; false_conv eq
+  case lam1 => intro eq; false_conv eq
+  case app0 => intro _ vl; cases vl
+  case app1 => intro _ vl; cases vl
+  case sig0 => intro eq; false_conv eq
+  case sig1 => intro eq; false_conv eq
+  case tup0 => intro eq; false_conv eq
+  case tup1 => intro eq; false_conv eq
+  case proj0 => intro _ vl; cases vl
+  case proj1 => intro _ vl; cases vl
   case bool => intro eq; false_conv eq
   case tt => intro eq; false_conv eq
   case ff => intro eq; false_conv eq
@@ -146,43 +247,74 @@ theorem Typed.progress {m A : Tm Srt} :
   all_goals try trivial
   case srt => right; constructor
   case var => right; constructor
-  case pi => right; constructor
-  case lam => right; constructor
-  case app _ n _ _ tym tyn ihm ihn =>
+  case pi0 => right; constructor
+  case pi1 => right; constructor
+  case lam0 => right; constructor
+  case lam1 => right; constructor
+  case app0 _ n _ tym tyn ihm ihn =>
     subst_vars
     match ihm (Eq.refl _) with
     | .inl ⟨m, _⟩ =>
       left; exists Tm.app m n
       constructor; assumption
     | .inr vl =>
-      have ⟨A, m, _⟩ := Typed.pi_canonical tym Conv.R vl
+      have ⟨A, m, _⟩ := tym.pi0_canonical Conv.R vl
       subst_vars
       left; exists m.[n/]
       constructor
-  case sig => right; constructor
-  case pair m n r s _ _ _ _ _ ihm ihn =>
+  case app1 _ n _ tym tyn ihm ihn =>
     subst_vars
-    match ihm (Eq.refl _), r with
-    | .inl ⟨m, _⟩, r =>
-      left; exists Tm.pair m n r s
+    match ihm (Eq.refl _) with
+    | .inl ⟨m, _⟩ =>
+      left; exists Tm.app m n
       constructor; assumption
-    | .inr vl, .im =>
+    | .inr vl =>
+      have ⟨A, m, _⟩ := tym.pi1_canonical Conv.R vl
+      subst_vars
+      left; exists m.[n/]
+      constructor
+  case sig0 => right; constructor
+  case sig1 => right; constructor
+  case tup0 m n s _ _ _ _ _ ihm ihn =>
+    subst_vars
+    match ihm (Eq.refl _) with
+    | .inl ⟨m, _⟩ =>
+      left; exists Tm.tup0 m n s
+      constructor; assumption
+    | .inr vl =>
       right; constructor; assumption
-    | .inr vl, .ex =>
+  case tup1 m n s _ _ _ _ _ ihm ihn =>
+    subst_vars
+    match ihm (Eq.refl _) with
+    | .inl ⟨m, _⟩ =>
+      left; exists Tm.tup1 m n s
+      constructor; assumption
+    | .inr vl =>
       match ihn (Eq.refl _) with
       | .inl ⟨n, _⟩ =>
-        left; exists Tm.pair m n .ex s
+        left; exists Tm.tup1 m n s
         constructor; assumption
       | .inr vl =>
         right; constructor <;> assumption
-  case proj C m n _ _ _ _ _ tym _ _ ihm _ =>
+  case proj0 C m n _ _ _ _ tym _ _ ihm _ =>
     subst_vars
     match ihm (Eq.refl _) with
     | .inl ⟨m, _⟩ =>
       left; exists Tm.proj C m n
       constructor; assumption
     | .inr vl =>
-      have ⟨m1, m2, _⟩ := Typed.sig_canonical tym Conv.R vl
+      have ⟨m1, m2, _⟩ := tym.sig0_canonical Conv.R vl
+      subst_vars
+      left; exists n.[m2,m1/]
+      constructor
+  case proj1 C m n _ _ _ _ tym _ _ ihm _ =>
+    subst_vars
+    match ihm (Eq.refl _) with
+    | .inl ⟨m, _⟩ =>
+      left; exists Tm.proj C m n
+      constructor; assumption
+    | .inr vl =>
+      have ⟨m1, m2, _⟩ := tym.sig1_canonical Conv.R vl
       subst_vars
       left; exists n.[m2,m1/]
       constructor
