SStructTT/Static/Step.lean
@@ -7,87 +7,115 @@ variable {Srt : Type}
 
 @[scoped aesop safe [constructors]]
 inductive Step : Tm Srt -> Tm Srt -> Prop where
-  | piA {A A'} B r s :
+  | pi0_A {A A'} B s :
     Step A A' ->
-    Step (.pi A B r s) (.pi A' B r s)
-  | piB A {B B'} r s :
+    Step (.pi0 A B s) (.pi0 A' B s)
+  | pi0_B A {B B'} s :
     Step B B' ->
-    Step (.pi A B r s) (.pi A B' r s)
-  | lamA {A A'} m r s :
+    Step (.pi0 A B s) (.pi0 A B' s)
+  | pi1_A {A A'} B s :
     Step A A' ->
-    Step (.lam A m r s) (.lam A' m r s)
-  | lamM A {m m'} r s :
+    Step (.pi1 A B s) (.pi1 A' B s)
+  | pi1_B A {B B'} s :
+    Step B B' ->
+    Step (.pi1 A B s) (.pi1 A B' s)
+  | lam0_A {A A'} m s :
+    Step A A' ->
+    Step (.lam0 A m s) (.lam0 A' m s)
+  | lam0_M A {m m'} s :
     Step m m' ->
-    Step (.lam A m r s) (.lam A m' r s)
-  | appM {m m'} n :
+    Step (.lam0 A m s) (.lam0 A m' s)
+  | lam1_A {A A'} m s :
+    Step A A' ->
+    Step (.lam1 A m s) (.lam1 A' m s)
+  | lam1_M A {m m'} s :
+    Step m m' ->
+    Step (.lam1 A m s) (.lam1 A m' s)
+  | app_M {m m'} n :
     Step m m' ->
     Step (.app m n) (.app m' n)
-  | appN m {n n'} :
+  | app_N m {n n'} :
     Step n n' ->
     Step (.app m n) (.app m n')
-  | beta A m n r s :
-    Step (.app (.lam A m r s) n) m.[n/]
-  | sigA {A A'} B r s :
+  | beta0 A m n s :
+    Step (.app (.lam0 A m s) n) m.[n/]
+  | beta1 A m n s :
+    Step (.app (.lam1 A m s) n) m.[n/]
+  | sig0_A {A A'} B s :
     Step A A' ->
-    Step (.sig A B r s) (.sig A' B r s)
-  | sigB A {B B'} r s :
+    Step (.sig0 A B s) (.sig0 A' B s)
+  | sig0_B A {B B'} s :
     Step B B' ->
-    Step (.sig A B r s) (.sig A B' r s)
-  | pairM {m m'} n r s :
+    Step (.sig0 A B s) (.sig0 A B' s)
+  | sig1_A {A A'} B s :
+    Step A A' ->
+    Step (.sig1 A B s) (.sig1 A' B s)
+  | sig1_B A {B B'} s :
+    Step B B' ->
+    Step (.sig1 A B s) (.sig1 A B' s)
+  | tup0_M {m m'} n s :
     Step m m' ->
-    Step (.pair m n r s) (.pair m' n r s)
-  | pairN m {n n'} r s :
+    Step (.tup0 m n s) (.tup0 m' n s)
+  | tup0_N m {n n'} s :
     Step n n' ->
-    Step (.pair m n r s) (.pair m n' r s)
-  | projA {A A'} m n :
+    Step (.tup0 m n s) (.tup0 m n' s)
+  | tup1_M {m m'} n s :
+    Step m m' ->
+    Step (.tup1 m n s) (.tup1 m' n s)
+  | tup1_N m {n n'} s :
+    Step n n' ->
+    Step (.tup1 m n s) (.tup1 m n' s)
+  | proj_A {A A'} m n :
     Step A A' ->
     Step (.proj A m n) (.proj A' m n)
-  | projM A {m m'} n :
+  | proj_M A {m m'} n :
     Step m m' ->
     Step (.proj A m n) (.proj A m' n)
-  | projN A m {n n'} :
+  | proj_N A m {n n'} :
     Step n n' ->
     Step (.proj A m n) (.proj A m n')
-  | projE A m1 m2 n r s :
-    Step (.proj A (.pair m1 m2 r s) n) n.[m2,m1/]
-  | iteA {A A'} m n1 n2 :
+  | proj0 A m1 m2 n s :
+    Step (.proj A (.tup0 m1 m2 s) n) n.[m2,m1/]
+  | proj1 A m1 m2 n s :
+    Step (.proj A (.tup1 m1 m2 s) n) n.[m2,m1/]
+  | ite_A {A A'} m n1 n2 :
     Step A A' ->
     Step (.ite A m n1 n2) (.ite A' m n1 n2)
-  | iteM A {m m'} n1 n2 :
+  | ite_M A {m m'} n1 n2 :
     Step m m' ->
     Step (.ite A m n1 n2) (.ite A m' n1 n2)
-  | iteN1 A m {n1 n1'} n2 :
+  | ite_N1 A m {n1 n1'} n2 :
     Step n1 n1' ->
     Step (.ite A m n1 n2) (.ite A m n1' n2)
-  | iteN2 A m n1 {n2 n2'} :
+  | ite_N2 A m n1 {n2 n2'} :
     Step n2 n2' ->
     Step (.ite A m n1 n2) (.ite A m n1 n2')
-  | iteT A n1 n2 :
+  | ite_true A n1 n2 :
     Step (.ite A .tt n1 n2) n1
-  | iteF A n1 n2 :
+  | ite_false A n1 n2 :
     Step (.ite A .ff n1 n2) n2
-  | idnA {A A'} m n :
+  | idn_A {A A'} m n :
     Step A A' ->
     Step (.idn A m n) (.idn A' m n)
-  | idnM A {m m'} n :
+  | idn_M A {m m'} n :
     Step m m' ->
     Step (.idn A m n) (.idn A m' n)
-  | idnN A m {n n'} :
+  | idn_N A m {n n'} :
     Step n n' ->
     Step (.idn A m n) (.idn A m n')
-  | rflM {m m'} :
+  | rfl_M {m m'} :
     Step m m' ->
     Step (.rfl m) (.rfl m')
-  | rwA {A A'} m n :
+  | rw_A {A A'} m n :
     Step A A' ->
     Step (.rw A m n) (.rw A' m n)
-  | rwM A {m m'} n :
+  | rw_M A {m m'} n :
     Step m m' ->
     Step (.rw A m n) (.rw A m' n)
-  | rwN A m {n n'} :
+  | rw_N A m {n n'} :
     Step n n' ->
     Step (.rw A m n) (.rw A m n')
-  | rwE A m n :
+  | rw_elim A m n :
     Step (.rw A m (.rfl n)) m
 
 abbrev StarStep := Star (@Step Srt)
