SStructTT/Dynamic/Typed.lean
@@ -1,0 +1,64 @@
+import SStructTT.Static.Typed
+import SStructTT.Dynamic.Context
+
+namespace Dynamic
+variable {Srt : Type} [inst : SStruct Srt]
+
+mutual
+inductive Typed : Static.Ctx Srt -> Dynamic.Ctx Srt -> Tm Srt -> Tm Srt -> Prop where
+  | var {Γ Δ x s A} :
+    Wf Γ Δ ->
+    Has Δ x s A ->
+    Typed Γ Δ (.var x) A
+  | lam0 {Γ Δ A B m} s :
+    Lower Δ s ->
+    Typed (A :: Γ) (_: Δ) m B ->
+    Typed Γ Δ (.lam0 A m s) (.pi0 A B s)
+  | lam1 {Γ Δ A B m} s :
+    Lower Δ s ->
+    Typed (A :: Γ) (A :⟨s⟩ Δ) m B ->
+    Typed Γ Δ (.lam1 A m s) (.pi1 A B s)
+  | app0 Γ Δ A B m n s :
+    Typed Γ Δ m (.pi0 A B s) ->
+    Γ ⊢ n : A ->
+    Typed Γ Δ (.app m n) B.[n/]
+  | app1 Γ Δ1 Δ2 Δ A B m n s :
+    Merge Δ1 Δ2 Δ ->
+    Typed Γ Δ1 m (.pi1 A B s) ->
+    Typed Γ Δ2 n A ->
+    Typed Γ Δ (.app m n) B.[n/]
+  | tup0 Γ Δ A B m n s i :
+    Γ ⊢ .sig0 A B s : .srt s i ->
+    Typed Γ Δ m A ->
+    Γ ⊢ n : B.[m/] ->
+    Typed Γ Δ (.tup0 m n s) (.sig0 A B s)
+  | tup1 Γ Δ1 Δ2 Δ A B m n s i :
+    Merge Δ1 Δ2 Δ ->
+    Γ ⊢ .sig1 A B s : .srt s i ->
+    Typed Γ Δ1 m A ->
+    Typed Γ Δ2 n B.[m/] ->
+    Typed Γ Δ (.tup1 m n s) (.sig1 A B s)
+  | proj0 Γ Δ1 Δ2 Δ A B C m n s1 s2 s3 i :
+    Merge Δ1 Δ2 Δ ->
+    (.sig A B t :: Γ) ⊢ C : Sort s l ->
+    Typed Γ Δ1 m (.sig A B .im t) ->
+    Typed (B :: A :: Γ) (_: A :⟨r⟩ Δ2) n C.[Pair0 (Var 1) (Var 0) t .: shift 2] ->
+    Typed Γ Δ (.proj C m n) C.[m/]
+  | dyn_letin1 Γ Δ1 Δ2 Δ A B C m n s r1 r2 t l :
+    Δ1 ∘ Δ2 => Δ ->
+    (Sig1 A B t :: Γ) ⊢ C : Sort s l ->
+    Γ ; Δ1 ⊢ m : Sig1 A B t ->
+    (B :: A :: Γ) ; B .{r2} A .{r1} Δ2 ⊢ n : C.[Pair1 (Var 1) (Var 0) t .: ren (+2)] ->
+    Γ ; Δ ⊢ LetIn C m n : C.[m/]
+
+inductive Wf : Static.Ctx Srt -> Dynamic.Ctx Srt -> Prop where
+  | nil : Wf [] []
+  | ex Γ Δ A s i :
+    Γ ⊢ A : .srt s i ->
+    Wf Γ Δ ->
+    Wf (A :: Γ) (A :⟨s⟩ Δ)
+  | im Γ Δ A s i :
+    Γ ⊢ A : .srt s i ->
+    Wf Γ Δ ->
+    Wf (A :: Γ) (_: Δ)
+end
