SStructTT/Static/Preservation.lean
@@ -12,25 +12,38 @@ theorem Typed.preservation {Γ : Ctx Srt} {A m n} :
   all_goals try trivial
   case srt => intro st; cases st
   case var => intro st; cases st
-  case pi ihA ihB =>
+  case pi0 ihA ihB =>
     intro st; cases st
-    case piA st =>
+    case pi0_A st =>
       constructor
       . apply ihA st
       . apply Typed.conv_ctx
         apply Conv.onei st
         apply ihA st
         assumption
-    case piB st =>
+    case pi0_B st =>
       constructor
       . assumption
       . apply ihB st
-  case lam tym ihA ihm =>
+  case pi1 ihA ihB =>
+    intro st; cases st
+    case pi1_A st =>
+      constructor
+      . apply ihA st
+      . apply Typed.conv_ctx
+        apply Conv.onei st
+        apply ihA st
+        assumption
+    case pi1_B st =>
+      constructor
+      . assumption
+      . apply ihB st
+  case lam0 tym ihA ihm =>
     have ⟨_, _, _⟩ := tym.validity
     intro st; cases st
-    case lamA st =>
+    case lam0_A st =>
       apply Typed.conv
-      . apply Conv.pi
+      . apply Conv.pi0
         apply Conv.onei st
         constructor
       . constructor
@@ -40,49 +53,106 @@ theorem Typed.preservation {Γ : Ctx Srt} {A m n} :
         apply ihA st
         assumption
       . constructor <;> assumption
-    case lamM st =>
+    case lam0_M st =>
       constructor
       . assumption
       . apply ihm st
-  case app tym tyn ihm ihn =>
-    have ⟨_, _, tyP⟩ := tym.validity
-    have ⟨_, _, _, tyB, _⟩ := tyP.pi_inv
+  case lam1 tym ihA ihm =>
+    have ⟨_, _, _⟩ := tym.validity
     intro st; cases st
-    case appM st =>
+    case lam1_A st =>
+      apply Typed.conv
+      . apply Conv.pi1
+        apply Conv.onei st
+        constructor
+      . constructor
+        apply ihA st
+        apply Typed.conv_ctx
+        apply Conv.onei st
+        apply ihA st
+        assumption
+      . constructor <;> assumption
+    case lam1_M st =>
       constructor
+      . assumption
+      . apply ihm st
+  case app0 tym tyn ihm ihn =>
+    have ⟨_, _, tyP⟩ := tym.validity
+    have ⟨_, _, _, tyB, _⟩ := tyP.pi0_inv
+    intro st; cases st
+    case app_M st =>
+      apply Typed.app0
       . apply ihm st
       . assumption
-    case appN st =>
+    case app_N st =>
       apply Typed.conv
       . apply Conv.subst1
         apply Conv.onei st
-      . constructor
+      . apply Typed.app0
         assumption
         apply ihn st
       . apply tyB.subst tyn
-    case beta =>
-      replace ⟨tym, _, _⟩ := tym.lam_inv; subst_vars
+    case beta0 =>
+      replace ⟨tym, _⟩ := tym.lam0_inv; subst_vars
       have ⟨_, _, _, tyA⟩ := tym.ctx_inv
       replace tyB := tyB.subst tyn; asimp at tyB
       apply tym.subst tyn
-  case sig ihA ihB =>
+    case beta1 =>
+      exfalso; apply tym.lam1_pi0_false; constructor
+  case app1 tym tyn ihm ihn =>
+    have ⟨_, _, tyP⟩ := tym.validity
+    have ⟨_, _, _, tyB, _⟩ := tyP.pi1_inv
     intro st; cases st
-    case sigA st =>
+    case app_M st =>
+      apply Typed.app1
+      . apply ihm st
+      . assumption
+    case app_N st =>
+      apply Typed.conv
+      . apply Conv.subst1
+        apply Conv.onei st
+      . apply Typed.app1
+        assumption
+        apply ihn st
+      . apply tyB.subst tyn
+    case beta0 =>
+      exfalso; apply tym.lam0_pi1_false; constructor
+    case beta1 =>
+      replace ⟨tym, _⟩ := tym.lam1_inv; subst_vars
+      have ⟨_, _, _, tyA⟩ := tym.ctx_inv
+      replace tyB := tyB.subst tyn; asimp at tyB
+      apply tym.subst tyn
+  case sig0 ihA ihB =>
+    intro st; cases st
+    case sig0_A st =>
       constructor
       . apply ihA st
       . apply Typed.conv_ctx
         apply Conv.onei st
         apply ihA st
         assumption
-    case sigB st =>
+    case sig0_B st =>
       constructor
       . assumption
       . apply ihB st
-  case pair tyS _ _ _ ihm ihn =>
+  case sig1 ihA ihB =>
     intro st; cases st
-    case pairM st =>
+    case sig1_A st =>
+      constructor
+      . apply ihA st
+      . apply Typed.conv_ctx
+        apply Conv.onei st
+        apply ihA st
+        assumption
+    case sig1_B st =>
+      constructor
+      . assumption
+      . apply ihB st
+  case tup0 tyS _ _ _ ihm ihn =>
+    intro st; cases st
+    case tup0_M st =>
       replace ihm := ihm st
-      have ⟨_, _, _, tyB, _⟩ := tyS.sig_inv
+      have ⟨_, _, _, tyB, _⟩ := tyS.sig0_inv
       constructor
       . assumption
       . assumption
@@ -91,22 +161,40 @@ theorem Typed.preservation {Γ : Ctx Srt} {A m n} :
         apply Conv.one st
         assumption
         apply tyB.subst ihm
-    case pairN st =>
+    case tup0_N st =>
       constructor
       . assumption
       . assumption
       . apply ihn st
-  case proj Γ A B C _ _ r s sC iC tyC tym tyn ihC ihm ihn =>
+  case tup1 tyS _ _ _ ihm ihn =>
+    intro st; cases st
+    case tup1_M st =>
+      replace ihm := ihm st
+      have ⟨_, _, _, tyB, _⟩ := tyS.sig1_inv
+      constructor
+      . assumption
+      . assumption
+      . apply Typed.conv
+        apply Conv.subst1
+        apply Conv.one st
+        assumption
+        apply tyB.subst ihm
+    case tup1_N st =>
+      constructor
+      . assumption
+      . assumption
+      . apply ihn st
+  case proj0 Γ A B C _ _ s sC iC tyC tym tyn ihC ihm ihn =>
     have ⟨s, _, wf, tyS⟩ := tyC.ctx_inv
-    have ⟨_, _, _, tyB, eq⟩ := tyS.sig_inv
+    have ⟨_, _, _, tyB, eq⟩ := tyS.sig0_inv
     have ⟨_, _, _, tyA⟩ := tyB.ctx_inv
     have ⟨_, _⟩ := Conv.srt_inj eq
     subst_vars; clear eq
     intro st; cases st
-    case projA C' st =>
+    case proj_A C' st =>
       replace ihC := ihC st
       have wf := tyn.toWf
-      have tyC' : (.sig A B r s).[shift 2] :: B :: A :: Γ ⊢ C'.[ren (upren (.+2))] :
+      have tyC' : (.sig0 A B s).[shift 2] :: B :: A :: Γ ⊢ C'.[ren (upren (.+2))] :
                   (.srt sC iC).[ren (upren (.+2))] := by
         apply Typed.renaming
         . assumption
@@ -114,10 +202,10 @@ theorem Typed.preservation {Γ : Ctx Srt} {A m n} :
           assumption
           rw[show (.+2) = (id !>> (.+1)) !>> (.+1) by funext; rfl]
           aesop (rule_sets := [rename])
-      have typ : B :: A :: Γ ⊢ .pair (.var 1) (.var 0) r s : (.sig A B r s).[shift 2] := by
-        asimp; apply Typed.pair
-        . rw[show Tm.sig A.[shift 2] B.[up (shift 2)] r s
-                = (Tm.sig A B r s).[shift 1].[shift 1] by asimp]
+      have typ : B :: A :: Γ ⊢ .tup0 (.var 1) (.var 0) s : (.sig0 A B s).[shift 2] := by
+        asimp; apply Typed.tup0
+        . rw[show Tm.sig0 A.[shift 2] B.[up (shift 2)] s
+                = (Tm.sig0 A B s).[shift 1].[shift 1] by asimp]
           have := (tyS.weaken tyA).weaken tyB
           assumption
         . rw[show A.[shift 2] = A.[shift 1].[shift 1] by asimp]
@@ -127,24 +215,81 @@ theorem Typed.preservation {Γ : Ctx Srt} {A m n} :
       apply Typed.conv
       . apply Conv.subst
         apply Conv.onei st
-      . apply Typed.proj ihC tym
+      . apply Typed.proj0 ihC tym
         apply Typed.conv
         apply Conv.subst
         apply Conv.one st
         assumption
         assumption
       . apply tyC.subst tym
-    case projM st =>
+    case proj_M st =>
       apply Typed.conv
       . apply Conv.subst1
         apply Conv.onei st
-      . apply Typed.proj tyC (ihm st) tyn
+      . apply Typed.proj0 tyC (ihm st) tyn
       . apply tyC.subst tym
-    case projN => constructor <;> aesop
-    case projE m1 m2 r s =>
-      have ⟨tym1, tym2, _, _⟩ := tym.pair_inv; subst_vars
-      rw[show C.[.pair m1 m2 r s/]
-            = C.[.pair (.var 1) (.var 0) r s .: shift 2].[m2,m1/] by asimp]
+    case proj_N => apply Typed.proj0 <;> aesop
+    case proj0 m1 m2 s =>
+      have ⟨tym1, tym2, _⟩ := tym.tup0_inv; subst_vars
+      rw[show C.[.tup0 m1 m2 s/]
+            = C.[.tup0 (.var 1) (.var 0) s .: shift 2].[m2,m1/] by asimp]
+      apply tyn.substitution
+      apply AgreeSubst.wk tym2
+      constructor; asimp; assumption
+      apply AgreeSubst.refl wf
+    case proj1 =>
+      exfalso; apply tym.tup1_sig0_false; constructor
+  case proj1 Γ A B C _ _ s sC iC tyC tym tyn ihC ihm ihn =>
+    have ⟨s, _, wf, tyS⟩ := tyC.ctx_inv
+    have ⟨_, _, _, tyB, eq⟩ := tyS.sig1_inv
+    have ⟨_, _, _, tyA⟩ := tyB.ctx_inv
+    have ⟨_, _⟩ := Conv.srt_inj eq
+    subst_vars; clear eq
+    intro st; cases st
+    case proj_A C' st =>
+      replace ihC := ihC st
+      have wf := tyn.toWf
+      have tyC' : (.sig1 A B s).[shift 2] :: B :: A :: Γ ⊢ C'.[ren (upren (.+2))] :
+                  (.srt sC iC).[ren (upren (.+2))] := by
+        apply Typed.renaming
+        . assumption
+        . apply AgreeRen.cons
+          assumption
+          rw[show (.+2) = (id !>> (.+1)) !>> (.+1) by funext; rfl]
+          aesop (rule_sets := [rename])
+      have typ : B :: A :: Γ ⊢ .tup1 (.var 1) (.var 0) s : (.sig1 A B s).[shift 2] := by
+        asimp; apply Typed.tup1
+        . rw[show Tm.sig1 A.[shift 2] B.[up (shift 2)] s
+                = (Tm.sig1 A B s).[shift 1].[shift 1] by asimp]
+          have := (tyS.weaken tyA).weaken tyB
+          assumption
+        . rw[show A.[shift 2] = A.[shift 1].[shift 1] by asimp]
+          constructor <;> aesop
+        . asimp; constructor <;> aesop
+      replace tyC' := tyC'.subst typ; asimp at tyC'; clear typ
+      apply Typed.conv
+      . apply Conv.subst
+        apply Conv.onei st
+      . apply Typed.proj1 ihC tym
+        apply Typed.conv
+        apply Conv.subst
+        apply Conv.one st
+        assumption
+        assumption
+      . apply tyC.subst tym
+    case proj_M st =>
+      apply Typed.conv
+      . apply Conv.subst1
+        apply Conv.onei st
+      . apply Typed.proj1 tyC (ihm st) tyn
+      . apply tyC.subst tym
+    case proj_N => apply Typed.proj1 <;> aesop
+    case proj0 =>
+      exfalso; apply tym.tup0_sig1_false; constructor
+    case proj1 m1 m2 s =>
+      have ⟨tym1, tym2, _⟩ := tym.tup1_inv; subst_vars
+      rw[show C.[.tup1 m1 m2 s/]
+            = C.[.tup1 (.var 1) (.var 0) s .: shift 2].[m2,m1/] by asimp]
       apply tyn.substitution
       apply AgreeSubst.wk tym2
       constructor; asimp; assumption
@@ -154,7 +299,7 @@ theorem Typed.preservation {Γ : Ctx Srt} {A m n} :
   case ff => intro st; cases st
   case ite tyA tym tyn1 tyn2 ihA ihm ihn1 ihn2 =>
     intro st; cases st
-    case iteA st =>
+    case ite_A st =>
       have wf := tym.toWf
       replace ihA := ihA st
       have tyAm := ihA.subst tym; asimp at tyAm
@@ -171,24 +316,24 @@ theorem Typed.preservation {Γ : Ctx Srt} {A m n} :
           apply Conv.subst
           apply Conv.one st
       . apply tyA.subst tym
-    case iteM st =>
+    case ite_M st =>
       apply Typed.conv
       . apply Conv.subst1
         apply Conv.onei st
       . constructor <;> try assumption
         apply ihm st
       . apply tyA.subst tym
-    case iteN1 st =>
+    case ite_N1 st =>
       constructor <;> try assumption
       apply ihn1 st
-    case iteN2 st =>
+    case ite_N2 st =>
       constructor <;> try assumption
       apply ihn2 st
-    case iteT => assumption
-    case iteF => assumption
+    case ite_true => assumption
+    case ite_false => assumption
   case idn ihA ihm ihn =>
     intro st; cases st
-    case idnA st =>
+    case idn_A st =>
       replace ihA := ihA st
       constructor
       . assumption
@@ -196,12 +341,12 @@ theorem Typed.preservation {Γ : Ctx Srt} {A m n} :
         apply Conv.one st
       . apply Typed.conv <;> try assumption
         apply Conv.one st
-    case idnM => constructor <;> aesop
-    case idnN => constructor <;> aesop
+    case idn_M => constructor <;> aesop
+    case idn_N => constructor <;> aesop
   case rfl tym ihm =>
     have ⟨_, _, _⟩ := tym.validity
     intro st; cases st
-    case rflM st =>
+    case rfl_M st =>
       apply Typed.conv
       . apply Conv.idn
         constructor
@@ -216,7 +361,7 @@ theorem Typed.preservation {Γ : Ctx Srt} {A m n} :
     have ⟨_, tya, _, _⟩ := tyI.idn_inv
     have ⟨_, _, _⟩ := tya.validity
     intro st; cases st
-    case rwA A' st =>
+    case rw_A A' st =>
       have : Γ ⊢ A'.[.rfl a, a/] : .srt s i := by
         rw[show .srt s i = (.srt s i).[.rfl a,a/] by asimp]
         apply Typed.substitution
@@ -246,8 +391,8 @@ theorem Typed.preservation {Γ : Ctx Srt} {A m n} :
         assumption
         assumption
       . assumption
-    case rwM st => constructor <;> aesop
-    case rwN n' st =>
+    case rw_M st => constructor <;> aesop
+    case rw_N n' st =>
       have : SConv (n' .: b .: ids) (n .: b .: ids) := by
         intro x; cases x with
         | zero => asimp; apply Conv.onei st
@@ -267,7 +412,7 @@ theorem Typed.preservation {Γ : Ctx Srt} {A m n} :
       . constructor <;> try assumption
         apply ihn st
       . assumption
-    case rwE c =>
+    case rw_elim c =>
       have ⟨_, eq1, eq2⟩ := tyn.rfl_inv
       have : SConv (.rfl a .: a .: ids) (.rfl c .: b .: ids) := by
         intro x; match x with
